src/Causal_CRDT.thy
@@ -199,7 +199,6 @@ apply clarsimp
 apply force
 done
 
-
 corollary (in finite_event_structure)
   shows "hb.hb_consistent (ordered_node_operations (carriers i))"
   apply(subgoal_tac "carriers i = [] \<or> (\<exists>c. carriers i = [c]) \<or> (length (carriers i) \<ge> 2)")
@@ -209,83 +208,8 @@ corollary (in finite_event_structure)
 defer
   apply(cases "carriers i"; clarsimp; case_tac "list"; clarsimp)
   apply(rule hb_consistent_technical[where i=i])
-  apply(subst carriers_compatible[symmetric])
+  apply(subst carriers_compatible)
   apply (rule horror_size3, simp+)
 done
 
-(*
-
-type_synonym lamport = "nat \<times> nat"
-
-datatype 'v operation
-  = Insert "lamport" "'v" "lamport option"
-
-locale network = finite_event_structure carriers
-    for carriers :: "nat \<Rightarrow> 'v operation event set" +
-  fixes event_id :: "'v operation event \<Rightarrow> lamport"
-  assumes event_id_unique: "event_id e1 = event_id e2 \<longleftrightarrow> e1 = e2"
-
-definition (in network) interpret_delivery :: "'v operation event \<Rightarrow> (lamport, 'v) elt list \<rightharpoonup> (lamport, 'v) elt list" where
-  "interpret_delivery oper_evt xs \<equiv>
-     case oper_evt of
-       (_, Deliver, Insert i v pos) \<Rightarrow> insert xs (i, v) pos
-     | (_, Broadcast, m) \<Rightarrow> Some xs"
-
-fun option_foldr :: "('a \<Rightarrow> 'b \<Rightarrow> 'b option) \<Rightarrow> 'a list \<Rightarrow> 'b \<Rightarrow> 'b option" where
-  "option_foldr f []     e = Some e" |
-  "option_foldr f (x#xs) e =
-     (case f x e of
-        None \<Rightarrow> None
-      | Some h \<Rightarrow> option_foldr f xs h)"
-
-lemma (in network) lengths_same:
-  assumes "{ m. (i, Deliver, m) \<in> carriers i } = { m. (j, Deliver, m) \<in> carriers j }"
-  shows   "length (ordered_node_operations i) = length (ordered_node_operations j)"
-using assms
-  apply(simp add: ordered_node_operations_def)
-  apply(rule finite.induct)
-  using finite_carriers sorry
-
-theorem (in network) foo:
-  assumes "{ m. (i, Deliver, m) \<in> carriers i } = { m. (j, Deliver, m) \<in> carriers j }"
-          "\<And>j lamp v pos. (j, Broadcast, Insert lamp v pos) \<in> carriers j \<Longrightarrow> pos = None \<or> (\<exists>k k' k''. pos = Some k \<and> (j, Deliver, Insert k k' k'') \<in> carriers j)"
-          "xs = ordered_node_operations i"
-          "ys = ordered_node_operations j"
-  shows   "option_foldr interpret_delivery xs [] =
-             option_foldr interpret_delivery ys []"
-using assms
-  apply(induction xs)
-  apply(drule lengths_same)
-  apply(simp add: ordered_node_operations_def)
-  apply(frule lengths_same, clarsimp)
-  apply(erule_tac x="i" in meta_allE)
-sorry
-
-definition next_lamport :: "(lamport, 'v) elt list \<Rightarrow> nat \<Rightarrow> lamport" where
-  "next_lamport xs node_name \<equiv>
-     let ss = fst ` fst ` set xs in
-       if ss = {} then
-         (node_name, 0)
-       else
-         (node_name, Suc (Max ss))"
-
-inductive possible_broadcasts :: "(lamport, 'v) elt list \<Rightarrow> nat \<Rightarrow> 'v operation event \<Rightarrow> bool" where
-  possible_broadcasts_Nil [intro!]: "\<lbrakk> next_lamport ([]::(lamport,'v) elt list) node_name = next \<rbrakk> \<Longrightarrow> possible_broadcasts [] node_name (node_name, Broadcast, (Insert next v None))" |
-  possible_broadcasts_Cons_tail [intro!]: "\<lbrakk> possible_broadcasts xs node_name tail \<rbrakk> \<Longrightarrow> possible_broadcasts (x#xs) node_name tail" |
-  possible_broadcasts_Cons_head [intro!]: "\<lbrakk> next_lamport xs node_name = next; (node_name, Broadcast, Insert next v (Some i)) = oper \<rbrakk> \<Longrightarrow> possible_broadcasts ((i,_)#xs) node_name oper"
-
-
-
-inductive node_state_evolution :: "(lamport, 'a) elt list \<Rightarrow> nat \<Rightarrow> 'a operation event \<Rightarrow> (lamport, 'a) elt list \<Rightarrow> bool" where
-  "\<lbrakk> interpret_delivery xs oper = Some ys \<rbrakk> \<Longrightarrow> node_state_evolution xs node_name (node_name, Deliver, oper) ys" |
-  "\<lbrakk> possible_broadcasts xs node_name ev \<rbrakk> \<Longrightarrow> node_state_evolution xs node_name ev xs"
-
-inductive (in node_state_evolution' :: "(lamport, 'a) elt list \<Rightarrow> 'a operation event set \<Rightarrow> (lamport, 'a) elt list \<Rightarrow> bool" where
-  "node_state_evolution' [] {} []" |
-  "\<lbrakk> node_state_evolution' xs es ys"
-
-locale infinite_stateful_network = infinite_event_structure +
-  fixes states :: "nat \<Rightarrow> (lamport, 'a) elt list"
-  
-*)
 end
